security/Backtranslation.v
@@ -304,7 +304,6 @@ Section CODEAUX.
         ge evres rt res
         (EVM: eventval_match ge evres (proj_rettype rt) res)
     :
-    (* (rettype_of_type (rettype_to_type rt)) = rt. *)
     proj_rettype (rettype_of_type (rettype_to_type rt)) = proj_rettype rt.
   Proof.
     inv EVM; destruct rt; simpl; auto.
@@ -508,8 +507,6 @@ Section GEN.
   Definition gen_counter_defs m (gds: list (ident * globdef Asm.fundef unit)): PTree.t (ident * globdef Clight.fundef type) :=
     let gds' := map (fun '(id, gd) => (id, (Pos.add id m, gen_counter (comp_of gd)))) gds in
     PTree_Properties.of_list gds'.
-  (* Definition gen_counter_defs m (gds: list (ident * globdef Asm.fundef unit)): PTree.t (ident * globdef Clight.fundef type) := *)
-  (*   fold_left (fun pt '(id, gd) => PTree.set id (Pos.add id m, gen_counter (comp_of gd)) pt) gds (@PTree.empty _). *)
 
   Definition params_of := PTree.t (list (ident * type)).
 
@@ -535,9 +532,6 @@ Section GEN.
                                          end) gds
     in
     PTree_Properties.of_list params'.
-  (* Definition gen_params (m: ident) (gds: list (ident * globdef Asm.fundef unit)): params_of := *)
-  (*   fold_left (fun pt '(id, gd) => *)
-  (*                match gen_params_one m gd with | Some ps => PTree.set id ps pt | None => pt end) gds (@PTree.empty _). *)
 
 
   Definition gen_progdef (ge: Senv.t) (tr: bundle_trace) a_gd (ocnt: option (ident * globdef Clight.fundef type)) (oparams: option (list (ident * type))): globdef Clight.fundef type :=
